

ALGORITHM BinarySearch ($A[0..n-1]$, n , x)

INPUT: Array A of n floating-point numbers, and target x

OUTPUT: Index i such that $A[i] = x$, or -1 if x not found

Iterative:

```
    low <- index of first element

    high <- index of last element          # define low and high bounds for
search space

    do:

        mid <- index of the "middle" element    # calculate the bisect (middle) of
the search space

        midVal <- A[mid]

        if (midVal == x):                    # found x, return now

            return mid;

        else:                                # didn't find x, divide and conquer from
here

            if (midVal < x):                  # remove the low-end (search space divided in half)

                low <- mid + 1                # search to the right of mid

            else:                             # remove the high-end (search space divided in
half)

                high <- mid - 1              # Search to the left of mid

        while:

            low <= high                      # run until low and high converge (no x is
found)

            return -1                        # no index was found
```

Recursive:

```
recursiveSearch(low <- index of first element, high <- index of last element):
```

```
    if (low >= high):                `      # run until low and high converge (no x is  
found)
```

```
        return -1                    # base case #1, no such element found
```

```
        mid <- index of the middle element      # calculate the bisect (middle) of the  
search space
```

```
        midVal <- A[mid]
```

```
    if (midVal == x):                # base case #2, x found at mid
```

```
        return mid
```

```
    else:                            # didn't find x, divide and conquer from  
here
```

```
        if (midVal < x):              # remove the low-end (search space divided in  
half)
```

```
            recursiveSearch(mid + 1, high) # Search to the right of mid
```

```
        else:                        # remove the high-end (search space  
divided in half)
```

```
            recursiveSearch(low, mid - 1)    # Search to the left of mid
```

ALGORITHM DoSomething(n)

INPUT: A positive integer n

OUTPUT: s, the summation of each element cubed in the set $\mathbb{Z}\{0\dots n\}$

```
IF n == 1                                     // base case
    return 1                                  // starts with 1
ELSE
    return DoSomething(n-1) + n * n * n // 1 + 2^3
                                           // 9 + 3^3
                                           // 36 + 4^3
                                           // 100 + 5^3
                                           // 225 + 6^3
                                           // 441 + 7^3...
```

Part 2.1:

This algorithm finds the summation of cubes for numbers n to 1;

The algorithm outputs s, the summation of each element cubed in the set $\mathbb{Z}\{0\dots n\}$

Part 2.2:

The Recursive Case:

$T() = T(n-1) + 1, T(1) = 1$ // $T(n-1)$ -> find each

Part 2.3:

// =====

// Recursive Case

// =====

$$T(n) = T(n-1) + 1$$

// =====

// 1st Occurence

// =====

$$\begin{aligned} T(n-1) &= T((n-1) - 1) + 1 + 1 \\ &= T(n-2) + 2 \end{aligned}$$

// =====

// 2nd Occurence

// =====

$$\begin{aligned} T(n-2) &= T((n-2) - 1) + 2 + 1 \\ &= T(n-3) + 3 \end{aligned}$$

// =====

// ith Occurence

// =====

$$T(n) = T(n-i) + i$$

// substitute $i = n - 1$ for the

$$= T(n - (n - 1)) + n - 1$$

$$= T(n - n + 1) + n - 1$$

```
// =====
```

```
// Closed Form
```

```
// =====
```

$$= T(1) + n - 1$$

```
// =====
```

```
// Time Complexity
```

```
// =====
```

$$T(n) = O(n)$$

Part 2.4:

The space complexity of the DoSomething algorithm is $O(n)$ because each recursion reduces n by 1 until the base case when n is 1, and each recursion only adds a single function to the heap.

Part 2.5:

ALGORITHM DoSomething(n)

INPUT: A positive integer n

OUTPUT: s , the summation of each element cubed in the set $\mathbb{Z} \{0 \dots n\}$

sum \rightarrow holds sum of all cubed n

IF $n > 1$ DO:

 sum += $n * n * n$;

$n--$;

return sum

Part 3.1:

1.

```
// =====
```

```
// Recurrence Relation
```

```
// =====
```

$$T(n) = T(n - 1) + n, T(1) = 1$$

```
// =====
```

```
// Recursive Case
```

```
// =====
```

$$T(n) = T(n - 1) + n$$

```
// =====
```

```
// 1st Occurrence
```

```
// =====
```

$$\begin{aligned} T(n) &= T((n - 1) - 1) + (n - 1) + n \\ &= T(n - 2) + (n - 1) + n \end{aligned}$$

```
// =====
```

```
// 2nd Occurrence
```

```
// =====
```

$$\begin{aligned} T(n) &= T((n - 2) - 1) + (n - 2) + (n - 1) + n \\ &= T(n - 3) + (n - 2) + (n - 1) + n \end{aligned}$$

```
// =====
```

```
// ith Occurrence
```

```
// =====
```

$T(n) = T(n - i) + \text{sum}(n - k) [\text{from } k = 0 \text{ to } i - 1]$

```
// =====
```

```
// Closed Form
```

```
// =====
```

```
// substitute  $i = n - 1 \Rightarrow n - i = 1$ 
```

$T(n) = T(1) + (1 + 2 + 3 + \dots + n)$

$= 1 + n(n + 1)/2$

```
// =====
```

```
// Time Complexity
```

```
// =====
```

$T(n) = O(n^2)$

2.

```
// =====
```

```
// Recurrence Relation
```

```
// =====
```

```
T(n) = 2T(n/2) + n, T(1) = 1
```

```
// =====
```

```
// Recursive Case
```

```
// =====
```

```
T(n) = 2T(n/2) + n
```

```
// =====
```

```
// 1st Occurrence
```

```
// =====
```

```
T(n) = 2(2T(n/2^2) + n/2) + n  
      = 2^2 T(n/2^2) + 2n
```

```
// =====
```

```
// 2nd Occurrence
```

```
// =====
```

```
T(n) = 2^3 T(n/2^3) + 3n
```

```
// =====
```

```
// ith Occurrence
```

```
// =====
```

```
T(n) = 2^i T(n/2^i) + i·n
```

```
// =====
```

```
// Closed Form
```

```
// =====
```

```
// substitute  $n/2^i = 1 \Rightarrow i = \log_2(n)$ 
```

$$T(n) = 2^{\log_2(n)} \cdot T(1) + n \log_2(n)$$

$$= n + n \log n$$

```
// =====
```

```
// Time Complexity
```

```
// =====
```

$$T(n) = O(n \log n)$$

3.

```
// =====
```

```
// Recurrence Relation
```

```
// =====
```

```
T(n) = 4T(n/2) + n2, T(1) = 1
```

```
// =====
```

```
// Recursive Case
```

```
// =====
```

```
T(n) = 4T(n/2) + n2
```

```
// =====
```

```
// 1st Occurrence
```

```
// =====
```

```
T(n) = 4(4T(n/22) + (n/2)2) + n2  
      = 42 T(n/22) + 2n2
```

```
// =====
```

```
// 2nd Occurrence
```

```
// =====
```

```
T(n) = 43 T(n/23) + 3n2
```

```
// =====
```

```
// ith Occurrence
```

```
// =====
```

```
T(n) = 4i T(n/2i) + sum(n2)[from j = 0 to i - 1]
```

```
// =====
```

```
// Closed Form
```

```
// =====
```

```
// substitute  $n/2^i = 1 \Rightarrow i = \log_2(n)$ 
```

```
 $T(n) = 4^{\log_2(n)} \cdot T(1) + n^2 \log_2(n)$ 
```

```
 $= n^2 + n^2 \log n$ 
```

```
// =====
```

```
// Time Complexity
```

```
// =====
```

```
 $T(n) = O(n^2 \log n)$ 
```

4.

```
// =====
```

```
// Recurrence Relation
```

```
// =====
```

```
T(n) = 8T(n/2) + 1, T(1) = 1
```

```
// =====
```

```
// Recursive Case
```

```
// =====
```

```
T(n) = 8T(n/2) + 1
```

```
// =====
```

```
// 1st Occurrence
```

```
// =====
```

```
T(n) = 8(8T(n/2^2) + 1) + 1
```

```
    = 8^2 T(n/2^2) + 9
```

```
// =====
```

```
// 2nd Occurrence
```

```
// =====
```

```
T(n) = 8^3 T(n/2^3) + (1 + 8 + 8^2)
```

```
// =====
```

```
// ith Occurrence
```

```
// =====
```

```
T(n) = 8^i T(n/2^i) + sum(8^j)[from j = 0 to i - 1]
```

```
// =====
```

```
// Closed Form
```

```
// =====
```

```
// substitute  $n/2^i = 1 \Rightarrow i = \log_2(n)$ 
```

```
 $T(n) = 8^{\log_2(n)} \cdot T(1) + O(8^{\log_2(n)})$ 
```

```
 $= n^3 + O(n^3)$ 
```

```
// =====
```

```
// Time Complexity
```

```
// =====
```

```
 $T(n) = O(n^3)$ 
```

5.

```
// =====
```

```
// Recurrence Relation
```

```
// =====
```

```
T(n) = 2T(n/2) + sqrt(n), T(1) = 1
```

```
// =====
```

```
// Recursive Case
```

```
// =====
```

```
T(n) = 2T(n/2) + sqrt(n)
```

```
// =====
```

```
// 1st Occurrence
```

```
// =====
```

```
T(n) = 2(2T(n/2^2) + sqrt(n/2)) + sqrt(n)
      = 2^2 T(n/2^2) + 2 sqrt(n/2) + sqrt(n)
```

```
// =====
```

```
// 2nd Occurrence
```

```
// =====
```

```
T(n) = 2^3 T(n/2^3) + 2^2 sqrt(n/2^2) + 2 sqrt(n/2) + sqrt(n)
```

```
// =====
```

```
// ith Occurrence
```

```
// =====
```

```
T(n) = 2^i T(n/2^i) + sum(2^j sqrt(n/2^j))[from j = 0 to i - 1]
```

// =====

// Closed Form

// =====

// substitute $n/2^i = 1 \Rightarrow i = \log_2(n)$

$$2^i T(1) = 2^{\log_2(n)} = n$$

$$2^j \sqrt{n/2^j} = \sqrt{n} \cdot 2^{j/2}$$

$$\sum(2^{j/2}) = O(2^{(\log n)/2}) = O(\sqrt{n})$$

$$T(n) = n + \sqrt{n} \cdot \sqrt{n}$$

$$= n + n$$

$$= 2n$$

// =====

// Time Complexity

// =====

$$T(n) = O(n)$$

Part 3.2:

1.

```
// =====  
  
// Recurrence Relation  
  
// =====  
  
 $T(n) = 2T(n/2) + n$   
  
  
  
// =====  
  
// Master Theorem Case  
  
// =====  
  
//  $T(n) = aT(n/b) + c \cdot n^k$   
//  $a = 2, b = 2, c = 1, k = 1$   
//  $T(1) = 1$   
//  $b^k = 2^1$   
//  $a = 2$   
// Case 2:  $a = b^k; T(n) = O(n^k \cdot \log(n))$   
//  $T(n) = O(n^1 \cdot \log(n))$   
  
  
// =====  
  
// Time Complexity  
  
// =====  
  
 $T(n) = O(n \cdot \log(n))$ 
```

2.

```
// =====  
  
// Recurrence Relation  
  
// =====  
  
 $T(n) = 4T(n/2) + n^2$   
  
  
// =====  
  
// Master Theorem  
  
// =====  
  
//  $T(n) = aT(n/b) + c \cdot n^k$   
  
//  $T(1) = c$   
  
//  $a = 4, b = 2, c = 1, k = 2$   
  
//  $T(1) = 1$   
  
//  $b^k = 2^2 = 4$   
  
//  $a = 4$   
  
// CASE 2:  $a = b^k; T(n) = O(n^k \cdot \log(n))$   
  
//  $T(n) = O(n^2 \cdot \log(n))$   
  
  
// =====  
  
// Time Complexity  
  
// =====  
  
 $T(n) = O(n^2 \cdot \log(n))$ 
```

3.

```
// =====  
  
// Recurrence Relation  
  
// =====  
  
 $T(n) = 8T(n/2) + 1$   
  
  
// =====  
  
// Master Theorem  
  
// =====  
  
//  $T(n) = aT(n/b) + c \cdot n^k$   
  
//  $T(1) = c$   
  
//  $a = 8, b = 2, c = 1, k = 1$   
  
//  $T(1) = 1$   
  
//  $b^k = 2^1 = 2$   
  
//  $a = 8$   
  
// CASE 3:  $a > b^k$   
  
//  $T(n) = O(n^{\log_2(8)}) = O(n^3)$   
  
  
// =====  
  
// Time Complexity  
  
// =====  
  
 $T(n) = O(n^3)$ 
```

4.

```
// =====  
  
// Recurrence Relation  
  
// =====  
  

$$T(n) = 2T(n/2) + \sqrt{n}$$
  
  
  
// =====  
  
// Master Theorem  
  
// =====  
  
//  $T(n) = aT(n/b) + c \cdot n^k$   
  
//  $T(1) = c$   
  
//  $a = 2, b = 2, c = 1, k = 1/2$   
  
//  $T(1) = 1$   
  
//  $b^k = \sqrt{2} = 2^{(1/2)}$   
  
//  $a = 2$   
  
// CASE 3:  $a > b^k$ ;  $T(n) = O(n^{\log_b(a)})$   
  
//  $T(n) = O(n^{\log_2(2)}) = O(n)$   
  
  
// =====  
  
// Time Complexity  
  
// =====  
  

$$T(n) = O(n)$$

```

5.

```
// =====  
  
// Recurrence Relation  
  
// =====  
  
 $T(n) = 9T(n/3) + n$   
  
  
// =====  
  
// Master Theorem  
  
// =====  
  
//  $T(n) = aT(n/b) + c \cdot n^k$   
  
//  $T(1) = c$   
  
//  $a = 9, b = 3, c = 1, k = 1$   
  
//  $T(1) = 1$   
  
//  $b^k = 3^1 = 3$   
  
//  $a = 9$   
  
// CASE 3:  $a > b^k$ ;  $T(n) = O(n^{\log_b(a)})$   
  
//  $T(n) = O(n^{\log_3(9)}) = O(n^2)$   
  
  
// =====  
  
// Time Complexity  
  
// =====  
  
 $T(n) = O(n^2)$ 
```

6.

```
// =====  
  
// Recurrence Relation  
  
// =====  
  
 $T(n) = T(2n/3) + 1$   
  
  
// =====  
  
// Master Theorem Case  
  
// =====  
  
//  $T(n) = aT(n/b) + c \cdot n^k$   
//  $a = 1, b = 2/3, c = 1, k = 0$   
//  $T(1) = 1$   
//  $b^k = 1$   
//  $a = 1$   
// Case 2:  $a = b^k; T(n) = O(n^k \cdot \log(n))$   
//  $T(n) = O(n^0 \cdot \log(n)) = O(\log(n))$   
  
  
// =====  
  
// Time Complexity  
  
// =====  
  
 $T(n) = O(\log(n))$ 
```